Work as of 15-05 13.53

AVL Tree.v
@@ -71,12 +71,12 @@ Fixpoint add (val:nat) (t: tree) :=
 
 Fixpoint balance (t : tree) :=
 	match t with
-	| leaf => leaf
+	| leaf => leaf (*Leaf tree is already balanced*)
 	| node val lChild rChild => 
 		match (height lChild) + 2 - (height rChild) with
-		| 0 => 
+		| 0 => (*-2, unbalanced to the right)
 			match rChild with
-			| leaf => leaf (* shouldn't happen *)
+			| leaf => leaf (* shouldn't happen with unbalance to the right *)
 			| node rval rlChild rrChild => 
 				match (height rlChild) + 2 - (height rrChild) with
 				| 1 => node rval (node val lChild rlChild) rrChild (* rr *)
@@ -88,7 +88,7 @@ Fixpoint balance (t : tree) :=
 					end
 				end
 			end
-		| 4 => 
+		| 4 => (*+2)
 			match lChild with
 			| leaf => leaf (* shouldn't happen *)
 			| node lval llChild lrChild => 
@@ -102,12 +102,21 @@ Fixpoint balance (t : tree) :=
 				| _ => node lval llChild (node val lrChild rChild) (* ll *)
 				end
 			end
-		| _ => node val (balance lChild) (balance rChild)
+		| _ => (*Rest should be -1, 0 and +1, which are balanced. Check on the rest of the tree.*)
+			node val (balance lChild) (balance rChild)
 		end
 	end.
 
 Definition insert val t :=
 	balance (add val t).
+
+Example insert_test :
+	insert 25 (insert 20 (insert 15 (insert 10 (insert 5 leaf)))) = node 10 (node 5 leaf leaf) (node 15 leaf (node 20 leaf leaf)).
+	(*node 15 (node 10 (node 5 leaf leaf) leaf) (node 20 leaf (node 25 leaf leaf)).*)
+	(*node 20 (node 10 (node 5 leaf leaf) (node 15 leaf leaf)) (node 25 leaf leaf).*)
+Proof.
+	compute. reflexivity.
+Qed.
 
 Fixpoint search (searchFor : nat) (t : tree) :=
 	match t with
@@ -430,7 +439,6 @@ Proof.
 			simpl in *. rewrite last_app_l. rewrite last_app_l in H0. apply last_inorder. apply IHt2. apply last_cons_le in H0. apply H0. apply H0.
 Qed.
 
-
 Theorem add_preserves_bst': forall n t,
 	sorted (inorder t) -> sorted (inorder (add n t)).
 Proof.
@@ -444,10 +452,61 @@ Proof.
 				apply IHt2. apply cons_sorted in H2. apply H2. congruence. 
 Qed.
 
+Lemma balance_inorder : forall t,
+	inorder t = inorder (balance t).
+Proof.
+	intros. induction t. 
+		Case "t = Leaf". reflexivity. 
+		Case "t = Node". simpl. remember (height t1 + 2 - height t2) as height1. destruct height1.
+			SCase "height1 = 0". destruct t2.
+				SSCase "t2 = Leaf". destruct t1. 
+					SSSCase "t1 = Leaf". inversion Heqheight1. 
+					SSSCase "t1 = Node". inversion Heqheight1.
+				SSCase "t2 = Node". remember (height t2_1 + 2 - height t2_2) as height2. destruct height2.
+					SSSCase "height2 = 0". destruct t2_1.
+						SSSSCase "t2_1 = Leaf". (* shouldn't happen *)destruct t2_2. 
+							SSSSSCase "t2_2 = Leaf". inversion Heqheight2. 
+							SSSSSCase "t2_2 = Node". simpl in Heqheight2. remember (max (height t2_2_1) (height t2_2_2)). destruct n2. 
+								inversion Heqheight2. 
+								simpl. admit.
+						SSSSCase "t2_1 = Node". simpl. repeat rewrite <- app_assoc. reflexivity.
+					SSSCase "height2 = S n". destruct height2.
+						SSSSCase "height2' = 0". simpl. repeat rewrite <- app_assoc. reflexivity.
+						SSSSCase "height2' = S n'". destruct t2_1.
+							SSSSSCase "t2_1 = Leaf". (* shouldn't happen *)simpl. simpl in Heqheight1, Heqheight2. remember (height t2_2). 
+								destruct n1. 
+									destruct height2. omega. omega.
+									destruct height2. 
+										destruct n1. omega. omega. 
+										destruct n1. omega. omega. 
+							SSSSSCase "t2_1 = Node". simpl. repeat rewrite <- app_assoc. reflexivity.
+			SCase "height1 = S n". destruct height1.
+				SSCase "height1' = 0". simpl. rewrite IHt1. rewrite IHt2. reflexivity.
+				SSCase "height1' = S n'". destruct height1.
+					SSSCase "height1'' = 0". simpl. rewrite IHt1. rewrite IHt2. reflexivity.
+					SSSCase "height1'' = S n''". destruct height1.
+						SSSSCase "height1''' = 0". simpl. rewrite IHt1, IHt2. reflexivity.
+						SSSSCase "height1''' = S n'''". simpl. destruct height1.
+							SSSSSCase "height1'''' = 0". destruct t1.
+								SSSSSSCase "t1 = Leaf". simpl in Heqheight1. remember (height t2). 
+									destruct n0. inversion Heqheight1. destruct n0. inversion Heqheight1. inversion Heqheight1. 
+								SSSSSSCase "t1 = Node". remember (height t1_1 + 2 - height t1_2) as height3. destruct height3.
+									SSSSSSSCase "height3 = 0". simpl. rewrite <- app_assoc. reflexivity.
+									SSSSSSSCase "height3 = S n". destruct height3.
+										(*height3' = 0*) destruct t1_2.
+											(*t1_2 = Leaf*) simpl in Heqheight3. omega. 
+											(*t1_2 = Node*) simpl. repeat rewrite <- app_assoc. simpl. rewrite <- app_assoc. reflexivity.
+										(*height3' = S n'*) simpl. repeat rewrite <- app_assoc. simpl. reflexivity.
+							SSSSSCase "height1'''' = S n''''". simpl. rewrite IHt1, IHt2. reflexivity.
+Qed.
+
 Theorem insert_preserves_bst : forall n t,
 	sorted (inorder t) -> sorted (inorder (insert n t)).
 Proof.
-	intros. induction t. 
+	intros. unfold insert. rewrite <- balance_inorder. apply add_preserves_bst'. assumption. 
+Qed.
+
+(*induction t. 
 		Case "t Leaf". simpl. apply single.
 		Case "t Node". simpl in H. apply sorted_app in H. inversion H. inversion H1. unfold insert. simpl in *. remember (ble_nat n n0) as add. 
 		destruct add. 
@@ -581,7 +640,7 @@ Proof.
 												(*height6' = S n'*)simpl. admit.
 									SSSSSSCase "height4'''' = S n''''". simpl. admit.
 	congruence.	
-Qed.
+Qed.*)
 
 Theorem insert_preserves_balance: forall n t t',
 	t = insert n t' ->height t <= log2 (length (inorder t') + 1) + 1 = true.
